LeanSAT/AIG/CachedGates.lean
@@ -1,37 +1,37 @@
 import LeanSAT.AIG.Cached
 import LeanSAT.AIG.CachedLemmas
 
-namespace Env
+namespace AIG
 
 /--
 Create a not gate in the input AIG. This uses the builtin cache to enable automated subterm sharing
 -/
-def mkNotCached (gate : Nat) (env : Env) (hgate : gate < env.decls.size) : Entrypoint :=
+def mkNotCached (gate : Nat) (aig : AIG) (hgate : gate < aig.decls.size) : Entrypoint :=
   -- ¬x = true && invert x
-  let constEntry := env.mkConstCached true
-  have := env.mkConstCached_le_size true
-  constEntry.env.mkGateCached
+  let constEntry := aig.mkConstCached true
+  have := aig.mkConstCached_le_size true
+  constEntry.aig.mkGateCached
     constEntry.start
     gate
     false
     true
     constEntry.inv
-    (by apply lt_mkConstCached_size_of_lt_env_size _ _ hgate)
+    (by apply lt_mkConstCached_size_of_lt_aig_size _ _ hgate)
 
 /--
 Create an and gate in the input AIG. This uses the builtin cache to enable automated subterm sharing
 -/
-def mkAndCached (lhs rhs : Nat) (env : Env) (hl : lhs < env.decls.size) (hr : rhs < env.decls.size) : Entrypoint :=
-  env.mkGateCached lhs rhs false false hl hr
+def mkAndCached (lhs rhs : Nat) (aig : AIG) (hl : lhs < aig.decls.size) (hr : rhs < aig.decls.size) : Entrypoint :=
+  aig.mkGateCached lhs rhs false false hl hr
 
 /--
 Create an or gate in the input AIG. This uses the builtin cache to enable automated subterm sharing
 -/
-def mkOrCached (lhs rhs : Nat) (env : Env) (hl : lhs < env.decls.size) (hr : rhs < env.decls.size) : Entrypoint :=
+def mkOrCached (lhs rhs : Nat) (aig : AIG) (hl : lhs < aig.decls.size) (hr : rhs < aig.decls.size) : Entrypoint :=
   -- x or y = true && (invert (invert x && invert y))
-  let auxEntry := env.mkGateCached lhs rhs true true hl hr
-  let constEntry := auxEntry.env.mkConstCached true
-  constEntry.env.mkGateCached
+  let auxEntry := aig.mkGateCached lhs rhs true true hl hr
+  let constEntry := auxEntry.aig.mkConstCached true
+  constEntry.aig.mkGateCached
     constEntry.start
     auxEntry.start
     false
@@ -42,41 +42,41 @@ def mkOrCached (lhs rhs : Nat) (env : Env) (hl : lhs < env.decls.size) (hr : rhs
 /--
 Create an xor gate in the input AIG. This uses the builtin cache to enable automated subterm sharing
 -/
-def mkXorCached (lhs rhs : Nat) (env : Env) (hl : lhs < env.decls.size) (hr : rhs < env.decls.size) : Entrypoint :=
+def mkXorCached (lhs rhs : Nat) (aig : AIG) (hl : lhs < aig.decls.size) (hr : rhs < aig.decls.size) : Entrypoint :=
   -- x xor y = (invert (invert (x && y))) && (invert ((invert x) && (invert y)))
-  let aux1Entry := env.mkGateCached lhs rhs false false hl hr
-  have := env.mkGateCached_le_size _ _ false false hl hr
-  have h3 : lhs < aux1Entry.env.decls.size := by
+  let aux1Entry := aig.mkGateCached lhs rhs false false hl hr
+  have := aig.mkGateCached_le_size _ _ false false hl hr
+  have h3 : lhs < aux1Entry.aig.decls.size := by
     dsimp [aux1Entry] at *
     omega
-  let aux2Entry := aux1Entry.env.mkGateCached
+  let aux2Entry := aux1Entry.aig.mkGateCached
       lhs
       rhs
       true
       true
       h3
-      (by apply lt_mkGateCached_size_of_lt_env_size; omega)
-  aux2Entry.env.mkGateCached aux1Entry.start aux2Entry.start true true (by apply lt_mkGateCached_size) aux2Entry.inv
+      (by apply lt_mkGateCached_size_of_lt_aig_size; omega)
+  aux2Entry.aig.mkGateCached aux1Entry.start aux2Entry.start true true (by apply lt_mkGateCached_size) aux2Entry.inv
 
 /--
 Create an equality gate in the input AIG. This uses the builtin cache to enable automated subterm sharing
 -/
-def mkBEqCached (lhs rhs : Nat) (env : Env) (hl : lhs < env.decls.size) (hr : rhs < env.decls.size) : Entrypoint :=
+def mkBEqCached (lhs rhs : Nat) (aig : AIG) (hl : lhs < aig.decls.size) (hr : rhs < aig.decls.size) : Entrypoint :=
   -- a == b = (invert (a && (invert b))) && (invert ((invert a) && b))
-  let aux1Entry := env.mkGateCached lhs rhs false true hl hr
-  have := env.mkGateCached_le_size _ _ false true hl hr
-  have h3 : lhs < aux1Entry.env.decls.size := by
+  let aux1Entry := aig.mkGateCached lhs rhs false true hl hr
+  have := aig.mkGateCached_le_size _ _ false true hl hr
+  have h3 : lhs < aux1Entry.aig.decls.size := by
     dsimp [aux1Entry] at *
     omega
   let aux2Entry :=
-    aux1Entry.env.mkGateCached
+    aux1Entry.aig.mkGateCached
       lhs
       rhs
       true
       false
       h3
-      (by apply lt_mkGateCached_size_of_lt_env_size; omega)
-  aux2Entry.env.mkGateCached
+      (by apply lt_mkGateCached_size_of_lt_aig_size; omega)
+  aux2Entry.aig.mkGateCached
     aux1Entry.start
     aux2Entry.start
     true
@@ -87,20 +87,20 @@ def mkBEqCached (lhs rhs : Nat) (env : Env) (hl : lhs < env.decls.size) (hr : rh
 /--
 Create an implication gate in the input AIG. This uses the builtin cache to enable automated subterm sharing
 -/
-def mkImpCached (lhs rhs : Nat) (env : Env) (hl : lhs < env.decls.size) (hr : rhs < env.decls.size) : Entrypoint :=
+def mkImpCached (lhs rhs : Nat) (aig : AIG) (hl : lhs < aig.decls.size) (hr : rhs < aig.decls.size) : Entrypoint :=
   -- a -> b = true && (invert (a and (invert b)))
   let auxEntry :=
-    env.mkGateCached
+    aig.mkGateCached
       lhs
       rhs
       false
       true
       hl
       hr
-  have := env.mkGateCached_le_size _ _ false true hl hr
-  let constEntry := mkConstCached true auxEntry.env
-  have := auxEntry.env.mkConstCached_le_size true
-  constEntry.env.mkGateCached
+  have := aig.mkGateCached_le_size _ _ false true hl hr
+  let constEntry := mkConstCached true auxEntry.aig
+  have := auxEntry.aig.mkConstCached_le_size true
+  constEntry.aig.mkGateCached
     constEntry.start
     auxEntry.start
     false
@@ -108,4 +108,4 @@ def mkImpCached (lhs rhs : Nat) (env : Env) (hl : lhs < env.decls.size) (hr : rh
     constEntry.inv
     (by apply lt_mkConstCached_size)
 
-end Env
+end AIG
