LeanSAT/AIG/Lemmas.lean
@@ -1,7 +1,7 @@
 import LeanSAT.Reflect.Tactics.Reflect
 import LeanSAT.AIG.Basic
 
-namespace Env
+namespace AIG
 
 /--
 `decls` is a prefix of `decls2`
@@ -28,7 +28,7 @@ theorem IsPrefix.of {decls1 decls2 : Array Decl}
 If `decls1` is a prefix of `decls2` and we start evaluating `decls2` at an
 index in bounds of `decls1` we can evluate at `decls1`.
 -/
-theorem denote.go_eq_of_env_eq (decls1 decls2 : Array Decl) (start : Nat) {hdag1} {hdag2}
+theorem denote.go_eq_of_aig_eq (decls1 decls2 : Array Decl) (start : Nat) {hdag1} {hdag2}
     {hbounds1} {hbounds2} (hprefix : IsPrefix decls1 decls2) :
     denote.go start decls2 assign hbounds2 hdag2
       =
@@ -54,17 +54,17 @@ theorem denote.go_eq_of_env_eq (decls1 decls2 : Array Decl) (start : Nat) {hdag1
       apply ReflectSat.EvalAtAtoms.and_congr
       all_goals
         apply ReflectSat.EvalAtAtoms.xor_congr
-        . apply denote.go_eq_of_env_eq
+        . apply denote.go_eq_of_aig_eq
           assumption
         . rfl
 termination_by sizeOf start
 
 /--
-Running `Env.denote.go` on a node that is within bounds of `decls` is equivalent to running it a bigger `decls` array.
+Running `AIG.denote.go` on a node that is within bounds of `decls` is equivalent to running it a bigger `decls` array.
 -/
 theorem denote.go_lt_push (x : Nat) (decls : Array Decl) {h1} {h2} {h3} :
     (denote.go x (decls.push decl) assign (by simp; omega) h3) = (denote.go x decls assign h1 h2)  := by
-  apply denote.go_eq_of_env_eq
+  apply denote.go_eq_of_aig_eq
   apply IsPrefix.of
   . intro idx h
     simp only [Array.get_push]
@@ -73,34 +73,34 @@ theorem denote.go_lt_push (x : Nat) (decls : Array Decl) {h1} {h2} {h3} :
     . contradiction
   . simp_arith
 
-@[inherit_doc denote.go_eq_of_env_eq ]
-theorem denote.eq_of_env_eq (entry : Entrypoint) (newEnv : Env) (hprefix : IsPrefix entry.env.decls newEnv.decls) :
-    ⟦newEnv, ⟨entry.start, (by have := entry.inv; have := hprefix.size_le; omega)⟩, assign⟧
+@[inherit_doc denote.go_eq_of_aig_eq ]
+theorem denote.eq_of_aig_eq (entry : Entrypoint) (newAIG : AIG) (hprefix : IsPrefix entry.aig.decls newAIG.decls) :
+    ⟦newAIG, ⟨entry.start, (by have := entry.inv; have := hprefix.size_le; omega)⟩, assign⟧
       =
     ⟦entry, assign⟧
     := by
   unfold denote
-  apply denote.go_eq_of_env_eq
+  apply denote.go_eq_of_aig_eq
   assumption
 
 @[simp]
-theorem denote_projected_entry {entry : Env.Entrypoint} :
-    ⟦entry.env, ⟨entry.start, entry.inv⟩, assign⟧ = ⟦entry, assign⟧ := by
+theorem denote_projected_entry {entry : AIG.Entrypoint} :
+    ⟦entry.aig, ⟨entry.start, entry.inv⟩, assign⟧ = ⟦entry, assign⟧ := by
   cases entry; simp
 
 /--
-`Env.mkGate` never shrinks the underlying AIG.
+`AIG.mkGate` never shrinks the underlying AIG.
 -/
-theorem mkGate_le_size (env : Env) (lhs rhs : Nat) (linv rinv : Bool) (hl) (hr)
-    : env.decls.size ≤ (env.mkGate lhs rhs linv rinv hl hr).env.decls.size := by
+theorem mkGate_le_size (aig : AIG) (lhs rhs : Nat) (linv rinv : Bool) (hl) (hr)
+    : aig.decls.size ≤ (aig.mkGate lhs rhs linv rinv hl hr).aig.decls.size := by
   simp_arith [mkGate]
 
 /--
-The AIG produced by `Env.mkGate` agrees with the input AIG on all indices that are valid for both.
+The AIG produced by `AIG.mkGate` agrees with the input AIG on all indices that are valid for both.
 -/
-theorem mkGate_decl_eq idx (env : Env) (lhs rhs : Nat) (linv rinv : Bool) {h : idx < env.decls.size} {hl} {hr} :
-    have := mkGate_le_size env lhs rhs linv rinv hl hr
-    (env.mkGate lhs rhs linv rinv hl hr).env.decls[idx]'(by omega) = env.decls[idx] := by
+theorem mkGate_decl_eq idx (aig : AIG) (lhs rhs : Nat) (linv rinv : Bool) {h : idx < aig.decls.size} {hl} {hr} :
+    have := mkGate_le_size aig lhs rhs linv rinv hl hr
+    (aig.mkGate lhs rhs linv rinv hl hr).aig.decls[idx]'(by omega) = aig.decls[idx] := by
   simp only [mkGate, Array.get_push]
   split
   . rfl
@@ -109,8 +109,8 @@ theorem mkGate_decl_eq idx (env : Env) (lhs rhs : Nat) (linv rinv : Bool) {h : i
 /--
 The input AIG to an `mkGate` is a prefix to the output AIG.
 -/
-theorem mkGate_IsPrefix_env (env : Env) (lhs rhs : Nat) (linv rinv : Bool) {hl} {hr} :
-    IsPrefix env.decls (env.mkGate lhs rhs linv rinv hl hr).env.decls := by
+theorem mkGate_IsPrefix_aig (aig : AIG) (lhs rhs : Nat) (linv rinv : Bool) {hl} {hr} :
+    IsPrefix aig.decls (aig.mkGate lhs rhs linv rinv hl hr).aig.decls := by
   apply IsPrefix.of
   . intro idx h
     apply mkGate_decl_eq
@@ -118,9 +118,9 @@ theorem mkGate_IsPrefix_env (env : Env) (lhs rhs : Nat) (linv rinv : Bool) {hl} 
 
 @[simp]
 theorem denote_mkGate :
-    ⟦env.mkGate lhs rhs linv rinv hl hr, assign⟧
+    ⟦aig.mkGate lhs rhs linv rinv hl hr, assign⟧
       =
-    ((xor ⟦env, ⟨lhs, hl⟩, assign⟧ linv) && (xor ⟦env, ⟨rhs, hr⟩, assign⟧ rinv)) := by
+    ((xor ⟦aig, ⟨lhs, hl⟩, assign⟧ linv) && (xor ⟦aig, ⟨rhs, hr⟩, assign⟧ rinv)) := by
   conv =>
     lhs
     unfold denote denote.go
@@ -140,74 +140,74 @@ theorem denote_mkGate :
       apply ReflectSat.EvalAtAtoms.xor_congr
       . unfold denote
         simp only [heq1, heq2]
-        apply denote.go_eq_of_env_eq
-        apply mkGate_IsPrefix_env
+        apply denote.go_eq_of_aig_eq
+        apply mkGate_IsPrefix_aig
       . simp only [heq3, heq4]
 
 /--
 We can show that something is < the output AIG of `mkGate` by showing that it is < the input AIG.
 -/
-theorem lt_mkGate_size_of_lt_env_size (env : Env) (lhs rhs : Nat) (linv rinv : Bool) (hl) (hr) (h : x < env.decls.size)
-    : x < (env.mkGate lhs rhs linv rinv hl hr).env.decls.size := by
-  have := mkGate_le_size env lhs rhs linv rinv hl hr
+theorem lt_mkGate_size_of_lt_aig_size (aig : AIG) (lhs rhs : Nat) (linv rinv : Bool) (hl) (hr) (h : x < aig.decls.size)
+    : x < (aig.mkGate lhs rhs linv rinv hl hr).aig.decls.size := by
+  have := mkGate_le_size aig lhs rhs linv rinv hl hr
   omega
 
 /--
-Reusing an `Env.Entrypoint` to build an additional gate will never invalidate the entry node of
+Reusing an `AIG.Entrypoint` to build an additional gate will never invalidate the entry node of
 the original entrypoint.
 -/
 theorem lt_mkGate_size (entry : Entrypoint) (lhs rhs : Nat) (linv rinv : Bool) (hl) (hr)
-    : entry.start < (entry.env.mkGate lhs rhs linv rinv hl hr).env.decls.size := by
-  apply lt_mkGate_size_of_lt_env_size
+    : entry.start < (entry.aig.mkGate lhs rhs linv rinv hl hr).aig.decls.size := by
+  apply lt_mkGate_size_of_lt_aig_size
   exact entry.inv
 
 /--
 We can show that something is ≤ the output AIG of `mkGate` by showing that it is ≤ the input AIG.
 -/
-theorem le_mkGate_size_of_le_env_size (env : Env) (lhs rhs : Nat) (linv rinv : Bool) (hl) (hr) (h : x ≤ env.decls.size)
-    : x ≤ (env.mkGate lhs rhs linv rinv hl hr).env.decls.size := by
-  have := mkGate_le_size env lhs rhs linv rinv hl hr
+theorem le_mkGate_size_of_le_aig_size (aig : AIG) (lhs rhs : Nat) (linv rinv : Bool) (hl) (hr) (h : x ≤ aig.decls.size)
+    : x ≤ (aig.mkGate lhs rhs linv rinv hl hr).aig.decls.size := by
+  have := mkGate_le_size aig lhs rhs linv rinv hl hr
   omega
 
 @[simp]
 theorem denote_mkGate_entry (entry : Entrypoint) {hlbound} {hrbound} {h} :
-    ⟦(entry.env.mkGate lhs rhs lpol rpol hlbound hrbound).env, ⟨entry.start, h⟩, assign ⟧
+    ⟦(entry.aig.mkGate lhs rhs lpol rpol hlbound hrbound).aig, ⟨entry.start, h⟩, assign ⟧
       =
     ⟦entry, assign⟧ :=  by
-  apply denote.eq_of_env_eq
-  apply mkGate_IsPrefix_env
+  apply denote.eq_of_aig_eq
+  apply mkGate_IsPrefix_aig
 
 @[simp]
 theorem denote_mkGate_lhs (entry : Entrypoint) {hlbound} {hrbound} {h} :
-    ⟦(entry.env.mkGate lhs rhs lpol rpol hlbound hrbound).env, ⟨lhs, h⟩, assign⟧
+    ⟦(entry.aig.mkGate lhs rhs lpol rpol hlbound hrbound).aig, ⟨lhs, h⟩, assign⟧
       =
-    ⟦entry.env, ⟨lhs, hlbound⟩, assign⟧ :=  by
-  apply denote.go_eq_of_env_eq
-  apply mkGate_IsPrefix_env
+    ⟦entry.aig, ⟨lhs, hlbound⟩, assign⟧ :=  by
+  apply denote.go_eq_of_aig_eq
+  apply mkGate_IsPrefix_aig
   . assumption
   . assumption
 
 @[simp]
 theorem denote_mkGate_rhs (entry : Entrypoint) {hlbound} {hrbound} {h} :
-    ⟦(entry.env.mkGate lhs rhs lpol rpol hlbound hrbound).env, ⟨rhs, h⟩, assign⟧
+    ⟦(entry.aig.mkGate lhs rhs lpol rpol hlbound hrbound).aig, ⟨rhs, h⟩, assign⟧
       =
-    ⟦entry.env, ⟨rhs, hrbound⟩, assign⟧ :=  by
-  apply denote.go_eq_of_env_eq
-  apply mkGate_IsPrefix_env
+    ⟦entry.aig, ⟨rhs, hrbound⟩, assign⟧ :=  by
+  apply denote.go_eq_of_aig_eq
+  apply mkGate_IsPrefix_aig
   . assumption
   . assumption
 
 /--
-`Env.mkAtom` never shrinks the underlying AIG.
+`AIG.mkAtom` never shrinks the underlying AIG.
 -/
-theorem mkAtom_le_size (env : Env) (var : Nat) : env.decls.size ≤ (env.mkAtom var).env.decls.size := by
+theorem mkAtom_le_size (aig : AIG) (var : Nat) : aig.decls.size ≤ (aig.mkAtom var).aig.decls.size := by
   simp_arith [mkAtom]
 
 /--
-The AIG produced by `Env.mkAtom` agrees with the input AIG on all indices that are valid for both.
+The AIG produced by `AIG.mkAtom` agrees with the input AIG on all indices that are valid for both.
 -/
-theorem mkAtom_decl_eq (env : Env) (var : Nat) (idx : Nat) {h : idx < env.decls.size} {hbound} :
-    (env.mkAtom var).env.decls[idx]'hbound = env.decls[idx] := by
+theorem mkAtom_decl_eq (aig : AIG) (var : Nat) (idx : Nat) {h : idx < aig.decls.size} {hbound} :
+    (aig.mkAtom var).aig.decls[idx]'hbound = aig.decls[idx] := by
   simp only [mkAtom, Array.get_push]
   split
   . rfl
@@ -216,16 +216,16 @@ theorem mkAtom_decl_eq (env : Env) (var : Nat) (idx : Nat) {h : idx < env.decls.
 /--
 The input AIG to an `mkAtom` is a prefix to the output AIG.
 -/
-theorem mkAtom_IsPrefix_env (env : Env) (var : Nat) :
-    IsPrefix env.decls (env.mkAtom var).env.decls := by
+theorem mkAtom_IsPrefix_aig (aig : AIG) (var : Nat) :
+    IsPrefix aig.decls (aig.mkAtom var).aig.decls := by
   apply IsPrefix.of
   . intro idx h
     apply mkAtom_decl_eq
   . apply mkAtom_le_size
 
 @[simp]
-theorem denote_mkAtom {env : Env} :
-    ⟦(env.mkAtom var), assign⟧ = assign var := by
+theorem denote_mkAtom {aig : AIG} :
+    ⟦(aig.mkAtom var), assign⟧ = assign var := by
   unfold denote denote.go
   split
   . next heq =>
@@ -241,25 +241,25 @@ theorem denote_mkAtom {env : Env} :
 
 @[simp]
 theorem denote_mkAtom_lt (entry : Entrypoint) {h} :
-    ⟦(entry.env.mkAtom var).env, ⟨entry.start, h⟩, assign⟧
+    ⟦(entry.aig.mkAtom var).aig, ⟨entry.start, h⟩, assign⟧
       =
     ⟦entry, assign⟧ := by
-  apply denote.eq_of_env_eq
-  apply mkAtom_IsPrefix_env
+  apply denote.eq_of_aig_eq
+  apply mkAtom_IsPrefix_aig
 
 /--
-`Env.mkConst` never shrinks the underlying AIG.
+`AIG.mkConst` never shrinks the underlying AIG.
 -/
-theorem mkConst_le_size (env : Env) (val : Bool)
-    : env.decls.size ≤ (env.mkConst val).env.decls.size := by
+theorem mkConst_le_size (aig : AIG) (val : Bool)
+    : aig.decls.size ≤ (aig.mkConst val).aig.decls.size := by
   simp_arith [mkConst]
 
 /--
-The AIG produced by `Env.mkConst` agrees with the input AIG on all indices that are valid for both.
+The AIG produced by `AIG.mkConst` agrees with the input AIG on all indices that are valid for both.
 -/
-theorem mkConst_decl_eq (env : Env) (val : Bool) (idx : Nat) {h : idx < env.decls.size} :
-    have := mkConst_le_size env val
-    (env.mkConst val).env.decls[idx]'(by omega) = env.decls[idx] := by
+theorem mkConst_decl_eq (aig : AIG) (val : Bool) (idx : Nat) {h : idx < aig.decls.size} :
+    have := mkConst_le_size aig val
+    (aig.mkConst val).aig.decls[idx]'(by omega) = aig.decls[idx] := by
   simp only [mkConst, Array.get_push]
   split
   . rfl
@@ -268,15 +268,15 @@ theorem mkConst_decl_eq (env : Env) (val : Bool) (idx : Nat) {h : idx < env.decl
 /--
 The input AIG to an `mkConst` is a prefix to the output AIG.
 -/
-theorem mkConst_IsPrefix_env (env : Env) (const : Bool) :
-    IsPrefix env.decls (env.mkConst const).env.decls := by
+theorem mkConst_IsPrefix_aig (aig : AIG) (const : Bool) :
+    IsPrefix aig.decls (aig.mkConst const).aig.decls := by
   apply IsPrefix.of
   . intro idx h
     apply mkConst_decl_eq
   . apply mkConst_le_size
 
 @[simp]
-theorem denote_mkConst {env : Env} : ⟦(env.mkConst val), assign⟧ = val := by
+theorem denote_mkConst {aig : AIG} : ⟦(aig.mkConst val), assign⟧ = val := by
   unfold denote denote.go
   split
   . next heq =>
@@ -292,60 +292,60 @@ theorem denote_mkConst {env : Env} : ⟦(env.mkConst val), assign⟧ = val := by
 
 @[simp]
 theorem denote_mkConst_entry (entry : Entrypoint) {h} :
-    ⟦(entry.env.mkConst val).env, ⟨entry.start, h⟩, assign⟧
+    ⟦(entry.aig.mkConst val).aig, ⟨entry.start, h⟩, assign⟧
       =
     ⟦entry, assign⟧ := by
-  apply denote.eq_of_env_eq
-  apply mkConst_IsPrefix_env
+  apply denote.eq_of_aig_eq
+  apply mkConst_IsPrefix_aig
 
 /--
 We can show that something is < the output AIG of `mkConst` by showing that it is < the input AIG.
 -/
-theorem lt_mkConst_size_of_lt_env_size (env : Env) (val : Bool) (h : x < env.decls.size) : x < (env.mkConst val).env.decls.size := by
-  have := mkConst_le_size env val
+theorem lt_mkConst_size_of_lt_aig_size (aig : AIG) (val : Bool) (h : x < aig.decls.size) : x < (aig.mkConst val).aig.decls.size := by
+  have := mkConst_le_size aig val
   omega
 
 /--
-Reusing an `Env.Entrypoint` to build an additional constant will never invalidate the entry node of
+Reusing an `AIG.Entrypoint` to build an additional constant will never invalidate the entry node of
 the original entrypoint.
 -/
-theorem lt_mkConst_size (entry : Entrypoint) (val : Bool) : entry.start < (entry.env.mkConst val).env.decls.size := by
-  apply lt_mkConst_size_of_lt_env_size
+theorem lt_mkConst_size (entry : Entrypoint) (val : Bool) : entry.start < (entry.aig.mkConst val).aig.decls.size := by
+  apply lt_mkConst_size_of_lt_aig_size
   exact entry.inv
 
 /--
 We can show that something is ≤ the output AIG of `mkConst` by showing that it is ≤ the input AIG.
 -/
-theorem le_mkConst_size_of_le_env_size (env : Env) (val : Bool) (h : x ≤ env.decls.size) : x ≤ (env.mkConst val).env.decls.size := by
-  have := mkConst_le_size env val
+theorem le_mkConst_size_of_le_aig_size (aig : AIG) (val : Bool) (h : x ≤ aig.decls.size) : x ≤ (aig.mkConst val).aig.decls.size := by
+  have := mkConst_le_size aig val
   omega
 
 /--
 If an index contains a `Decl.const` we know how to denote it.
 -/
-theorem denote_idx_const (h : env.decls[start] = .const b) :
-    ⟦env, ⟨start, hstart⟩, assign⟧ = b := by
+theorem denote_idx_const (h : aig.decls[start] = .const b) :
+    ⟦aig, ⟨start, hstart⟩, assign⟧ = b := by
   unfold denote denote.go
   split <;> simp_all
 
 /--
 If an index contains a `Decl.atom` we know how to denote it.
 -/
-theorem denote_idx_atom (h : env.decls[start] = .atom a) :
-    ⟦env, ⟨start, hstart⟩, assign⟧ = assign a := by
+theorem denote_idx_atom (h : aig.decls[start] = .atom a) :
+    ⟦aig, ⟨start, hstart⟩, assign⟧ = assign a := by
   unfold denote denote.go
   split <;> simp_all
 
 /--
 If an index contains a `Decl.gate` we know how to denote it.
 -/
-theorem denote_idx_gate (h : env.decls[start] = .gate lhs rhs linv rinv) :
-    ⟦env, ⟨start, hstart⟩, assign⟧
+theorem denote_idx_gate (h : aig.decls[start] = .gate lhs rhs linv rinv) :
+    ⟦aig, ⟨start, hstart⟩, assign⟧
       =
     (
-      (xor ⟦env, ⟨lhs, by have := env.inv start lhs rhs linv rinv hstart h; omega⟩, assign⟧ linv)
+      (xor ⟦aig, ⟨lhs, by have := aig.inv start lhs rhs linv rinv hstart h; omega⟩, assign⟧ linv)
         &&
-      (xor ⟦env, ⟨rhs, by have := env.inv start lhs rhs linv rinv hstart h; omega⟩, assign⟧ rinv)
+      (xor ⟦aig, ⟨rhs, by have := aig.inv start lhs rhs linv rinv hstart h; omega⟩, assign⟧ rinv)
     ) := by
   unfold denote
   conv =>
@@ -359,4 +359,4 @@ theorem denote_idx_gate (h : env.decls[start] = .gate lhs rhs linv rinv) :
     simp_all
 
 
-end Env
+end AIG
